wip mod2 bir contract

examples/riscv/mod2/mod2_propScript.sml
@@ -44,7 +44,11 @@ open mod2Theory;
 
 open mod2_symb_execTheory;
 
+open distribute_generic_stuffTheory;
+
 val _ = new_theory "mod2_prop";
+
+val birs_state_ss = rewrites (type_rws ``:birs_state_t``);
 
 (* --------------- *)
 (* RISC-V contract *)
@@ -80,6 +84,9 @@ Definition bir_mod2_post_def:
     (BExp_Const (Imm64 (n2w (x MOD 2))))
 End
 
+val bir_mod2_pre = ``bir_mod2_pre``;
+val bir_mod2_post = ``bir_mod2_post``;
+
 (* ----------------------------------- *)
 (* Connecting RISC-V and BIR contracts *)
 (* ----------------------------------- *)
@@ -99,6 +106,149 @@ QED
 (* ------------------------------- *)
 (* BIR symbolic execution analysis *)
 (* ------------------------------- *)
+
+val (sys_i, L_s, Pi_f) = (symb_sound_struct_get_sysLPi_fun o concl) mod2_symb_analysis_thm;
+
+Definition incr_analysis_L_def:
+ incr_analysis_L = ^(L_s)
+End
+
+val birs_state_init_lbl = ``<|bpc_label := BL_Address (Imm64 0w); bpc_index := 0|>``;
+val birs_state_end_lbl = (snd o dest_eq o concl o EVAL) ``bir_block_pc (BL_Address (Imm64 4w))``;
+
+Theorem mod2_analysis_L_NOTIN_thm[local]:
+  (^birs_state_end_lbl) NOTIN incr_analysis_L
+Proof
+  EVAL_TAC
+QED
+
+(* ........................... *)
+(* ........................... *)
+(* ........................... *)
+
+val birs_state_init_pre = ``birs_state_init_pre_GEN ^birs_state_init_lbl mod2_birenvtyl (mk_bsysprecond (bir_mod2_pre pre_x10) mod2_birenvtyl)``;
+
+val mod2_bsysprecond_thm = (computeLib.RESTR_EVAL_CONV [``birs_eval_exp``] THENC birs_stepLib.birs_eval_exp_CONV) ``mk_bsysprecond (bir_mod2_pre pre_x10) mod2_birenvtyl``;
+
+Theorem birs_state_init_pre_EQ_thm:
+  ^((snd o dest_comb) sys_i) = ^birs_state_init_pre
+Proof
+  REWRITE_TAC [birs_state_init_pre_GEN_def, mk_bsysprecond_def, mod2_bsysprecond_thm] >>
+  CONV_TAC (computeLib.RESTR_EVAL_CONV [``birs_eval_exp``] THENC birs_stepLib.birs_eval_exp_CONV)
+QED
+
+val mod2_analysis_thm =
+  REWRITE_RULE [birs_state_init_pre_EQ_thm, GSYM bir_mod2_prog_def] mod2_symb_analysis_thm;
+
+Theorem mod2_birenvtyl_EVAL_thm =
+ (REWRITE_CONV [mod2_birenvtyl_def,
+   bir_lifting_machinesTheory.riscv_bmr_vars_EVAL,
+   bir_lifting_machinesTheory.riscv_bmr_temp_vars_EVAL] THENC EVAL)
+ ``mod2_birenvtyl``;
+
+val birs_state_thm = REWRITE_CONV [mod2_birenvtyl_EVAL_thm] birs_state_init_pre;
+
+(* ------ *)
+
+(* now the transfer *)
+
+val bprog_tm = (fst o dest_eq o concl) bir_mod2_prog_def;
+
+val birs_symb_symbols_f_sound_prog_thm =
+  (SPEC (inst [Type`:'observation_type` |-> Type.alpha] bprog_tm) bir_symb_soundTheory.birs_symb_symbols_f_sound_thm);
+
+val birs_prop_transfer_thm =
+  (MATCH_MP symb_prop_transferTheory.symb_prop_transfer_thm birs_symb_symbols_f_sound_prog_thm);
+
+Definition bprog_P_def:
+  bprog_P x = P_bircont mod2_birenvtyl (^bir_mod2_pre x)
+End
+
+Definition bprog_Q_def:
+  bprog_Q x = Q_bircont (^birs_state_end_lbl) (set mod2_prog_vars) (^bir_mod2_post x)
+End
+
+Definition pre_bir_nL_def:
+  pre_bir_nL x = pre_bircont_nL mod2_birenvtyl (^bir_mod2_pre x)
+End
+
+Definition post_bir_nL_def:
+  post_bir_nL x = post_bircont_nL (^birs_state_end_lbl) (set mod2_prog_vars) (^bir_mod2_post x)
+End
+(* ........................... *)
+
+(* P is generic enough *)
+(* taken from "bir_exp_to_wordsLib" *)
+val type_of_bir_exp_thms =
+    let
+      open bir_immTheory
+      open bir_valuesTheory
+      open bir_envTheory
+      open bir_exp_memTheory
+      open bir_bool_expTheory
+      open bir_extra_expsTheory
+      open bir_nzcv_expTheory
+      open bir_interval_expTheory
+      in [
+        type_of_bir_exp_def,
+        bir_var_type_def,
+        bir_type_is_Imm_def,
+        type_of_bir_imm_def,
+        BExp_Aligned_type_of,
+        BExp_unchanged_mem_interval_distinct_type_of,
+        bir_number_of_mem_splits_REWRS,
+        BType_Bool_def,
+        bir_exp_true_def,
+        bir_exp_false_def,
+        BExp_MSB_type_of,
+        BExp_nzcv_ADD_DEFS,
+        BExp_nzcv_SUB_DEFS,
+        n2bs_def,
+        BExp_word_bit_def,
+        BExp_Align_type_of,
+        BExp_ror_type_of,
+        BExp_LSB_type_of,
+        BExp_word_bit_exp_type_of,
+        BExp_ADD_WITH_CARRY_type_of,
+        BExp_word_reverse_type_of,
+        BExp_ror_exp_type_of
+      ] end;
+
+Theorem bprog_P_entails_thm[local]:
+  P_entails_an_interpret (bir_symb_rec_sbir ^bprog_tm) (bprog_P pre_x10) (birs_symb_to_symbst ^birs_state_init_pre)
+Proof
+  ASSUME_TAC (GSYM mod2_prog_vars_thm) >>
+  `mod2_prog_vars = MAP PairToBVar mod2_birenvtyl` by (
+    SIMP_TAC std_ss [mod2_birenvtyl_def, listTheory.MAP_MAP_o, PairToBVar_BVarToPair_I_thm, listTheory.MAP_ID]
+  ) >>
+  POP_ASSUM (fn thm => FULL_SIMP_TAC std_ss [thm]) >>
+  IMP_RES_TAC (SIMP_RULE std_ss [] P_bircont_entails_thm) >>
+
+  SIMP_TAC std_ss [bprog_P_def] >>
+  POP_ASSUM (ASSUME_TAC o Q.SPEC `bir_mod2_pre pre_x10`) >>
+  `bir_vars_of_exp (bir_mod2_pre pre_x10) SUBSET set (MAP PairToBVar mod2_birenvtyl)` by (
+    PAT_X_ASSUM ``A = set B`` (fn thm => REWRITE_TAC [GSYM thm]) >>
+    SIMP_TAC (std_ss++holBACore_ss) [bir_mod2_pre_def, bir_mod2_pre_def] >>
+    SIMP_TAC (std_ss++pred_setLib.PRED_SET_ss) [GSYM mod2_prog_vars_thm, mod2_prog_vars_def, bir_mod2_pre_def] >>
+    SIMP_TAC (std_ss++pred_setLib.PRED_SET_ss++holBACore_ss) [listTheory.MEM, pred_setTheory.IN_INSERT]
+  ) >>
+  POP_ASSUM (fn thm => FULL_SIMP_TAC std_ss [thm]) >>
+  `ALL_DISTINCT (MAP FST mod2_birenvtyl)` by (
+    SIMP_TAC (std_ss++listSimps.LIST_ss) [mod2_birenvtyl_EVAL_thm]
+  ) >>
+  POP_ASSUM (fn thm => FULL_SIMP_TAC std_ss [thm]) >>
+  `IS_SOME (type_of_bir_exp (bir_mod2_pre pre_x10))` by (
+    SIMP_TAC std_ss [bir_mod2_pre_def, bir_mod2_pre_def] >>
+    CONV_TAC (RAND_CONV (SIMP_CONV (srw_ss()) type_of_bir_exp_thms)) >>
+    SIMP_TAC (std_ss++holBACore_ss) [optionTheory.option_CLAUSES]
+  ) >>
+  POP_ASSUM (fn thm => FULL_SIMP_TAC std_ss [thm])
+QED
+
+(* ........................... *)
+(* proof for each end state individually: *)
+
+(* -------------------- *)
 
 Theorem bir_cont_mod2[local]:
  bir_cont bir_mod2_prog bir_exp_true (BL_Address (Imm64 0w))
